tests/micro-benchmarks/TestWellFoundedRecursion.fst
@@ -209,3 +209,12 @@ let rec rel_poly (a:Type) (r:binrel a) (wf_r:well_founded (WFU.squash_binrel r))
     | None -> 0
     | Some z -> 
       1 + rel_poly a r wf_r (dsnd z)
+
+
+let rec rel_poly2 (a:Type) (r:binrel a) (wf_r:well_founded r) (x:a)
+  : Tot nat (decreases {:well-founded WFU.lift_binrel_as_well_founded_relation wf_r (| a, x |)})
+  = match get_previous (WFU.lift_binrel_as_well_founded_relation wf_r) (| a, x |) with
+    | None -> 0
+    | Some z ->
+      WFU.elim_lift_binrel r z x;
+      1 + rel_poly2 a r wf_r (dsnd z)
