ulib/FStar.WellFounded.Util.fsti
@@ -27,6 +27,8 @@ open FStar.WellFounded
 
       This is useful when writing type-polymorphic recursive functions
       whose termination depends on some custom well-founded order
+
+      See tests/micro-benchmarks/TestWellFoundedRecursion.rel_poly2
 *)
       
 let top = (b:Type & b)
@@ -36,6 +38,11 @@ let lift_binrel (#a:Type)
     : binrel top
     = fun (t0 t1:top) ->
         (_:(dfst t0==a /\ dfst t1==a) & r (dsnd t0) (dsnd t1))
+
+val elim_lift_binrel (#a:Type) (r:binrel a) (y:top) (x:a)
+  : Lemma 
+    (requires lift_binrel r y (| a, x |))
+    (ensures dfst y == a /\ r (dsnd y) x)
 
 val lower_binrel (#a:Type)
                  (#r:binrel a)
@@ -60,7 +67,11 @@ let lift_binrel_as_well_founded_relation (#a:Type u#a) (#r:binrel u#a u#r a) (wf
       in `a` by `r`
 
       This is very similar to 1, but uses squashed types,
-      which leads to better SMT automation at use sites *)
+      which leads to slightly better SMT automation at use sites.
+
+      See tests/micro-benchmarks/TestWellFoundedRecursion.rel_poly
+      
+*)
 let lift_binrel_squashed (#a:Type u#a)
                          (r:binrel u#a u#r a)
     : binrel top
